RState.v
@@ -1,0 +1,134 @@
+Require Export Coq.Init.Datatypes.
+Require Import Coq.Logic.ProofIrrelevance.
+Require Import Coq.Program.Basics.
+Require Import Coq.Program.Equality.
+Require Import Coq.Program.Tactics.
+Require Import Coq.Structures.Orders.
+Require Import FunctionalExtensionality.
+Require Import Endo.
+Require Import Applicative.
+Require Import Monad.
+Require Import Recdef.
+
+Open Scope program_scope.
+
+Section RState.
+
+Variable   s : Type.
+Hypothesis P : relation s.
+Context  `(e : PreOrder s P).
+
+Record StateP (before : s) (a : Type) := {
+    after  : s;
+    result : a;
+    holds  : P before after
+}.
+
+Arguments after [before] [a] _.
+Arguments result [before] [a] _.
+Arguments holds [before] [a] _.
+
+(** The [RState] monad requires that a given equivalence relation hold
+    between state transitions. *)
+Inductive RState (a : Type) : Type :=
+  | St : (forall st : s, StateP st a) -> RState a.
+
+Arguments St [a] _.
+
+Definition runRState {a : Type} (v : RState a)
+  : forall st : s, StateP st a :=
+      match v with St f => fun st => f st end.
+
+Definition RState_fmap (a b : Type) (f : a -> b) (x : RState a)
+  : RState b :=
+  St (fun st =>
+        let sp := runRState x st in
+        {| after  := after sp
+         ; result := f (result sp)
+         ; holds  := holds sp
+         |}).
+
+Hint Unfold RState_fmap.
+
+Ltac RState_auto :=
+  intros; simpl;
+  repeat (
+    autounfold; unfold id, compose; simpl;
+    f_equal; try apply proof_irrelevance; auto;
+    match goal with
+    | [ |- (fun _ : RState _ => _) = (fun _ : RState _ => _) ] =>
+        extensionality sx
+    | [ |- (fun _ : s => _) = _ ] =>
+        extensionality st
+    | [ st : s, sp : forall st : s, StateP st _ |- _ ] =>
+        destruct (sp st)
+    | [ sx : RState _ |- _ ] => destruct sx as [sp]
+    | [ |- St _ = St _ ] => f_equal
+    end).
+
+Obligation Tactic := RState_auto.
+
+Program Instance RState_Functor : Functor RState := {
+    fmap := RState_fmap
+}.
+
+Definition RState_pure (a : Type) (x : a) : RState a :=
+  St (fun st =>
+        {| after  := st
+         ; result := x
+         ; holds  := reflexivity st
+         |}).
+
+Hint Unfold RState_pure.
+
+Definition RState_ap (a b : Type) (f : RState (a -> b)) (x : RState a)
+  : RState b :=
+  St (fun st =>
+        let spf := runRState f st in
+        let spx := runRState x (after spf) in
+        {| after  := after spx
+         ; result := (result spf) (result spx)
+         ; holds  := transitivity (holds spf) (holds spx)
+         |}).
+
+Hint Unfold RState_ap.
+
+Program Instance RState_Applicative : Applicative RState := {
+    pure := RState_pure;
+    ap   := RState_ap
+}.
+
+Definition RState_join (a : Type) (x : RState (RState a)) : RState a :=
+  St (fun st =>
+        let sp := runRState x st in
+        let sp' := runRState (result sp) (after sp) in
+        {| after  := after sp'
+         ; result := result sp'
+         ; holds  := transitivity (holds sp) (holds sp')
+         |}).
+
+Hint Unfold RState_join.
+
+Program Instance RState_Monad : Monad RState := {
+    join := RState_join
+}.
+
+Definition get : RState s :=
+  St (fun st =>
+        {| after  := st
+         ; result := st
+         ; holds  := reflexivity st
+         |}).
+
+(** There cannot be a definition of [put], since we can only lawfully
+    transform the state, not simply replace it.  Therefore, [modify] must be
+    used in all cases where [put] would ordinarily have been. *)
+Definition modify (f : forall st : s, { st' : s & P st st' }) : RState unit :=
+  St (fun st =>
+        let (st', H) := f st in
+        {| after  := st'
+         ; result := tt
+         ; holds  := H
+         |}).
+
+End RState.
